src/Preservation.v
@@ -1,5 +1,6 @@
 Require Import EventCSL.
 Require Import Locking.
+Require Import ForwardChaining.
 Import List.
 Import List.ListNotations.
 
@@ -33,39 +34,51 @@ Definition preserves (R : S -> S -> Prop) F F' :=
     (F * P)%pred (proj s').
 
 Definition pred_domain F (dom: list AT) :=
+  (forall m, F m -> forall a v, m a = Some v -> In a dom) /\
+  (forall m, F m -> forall a, In a dom -> m a <> None).
+
+Lemma pred_domain_exists : forall F dom,
+  pred_domain F dom <->
   forall m, F m ->
   (forall a, (exists v, m a = Some v) <-> In a dom).
-
-Lemma pred_domain_universal : forall F dom,
-  pred_domain F dom <->
-  (forall m a v, F m -> m a = Some v -> In a dom) /\
-  (forall m a, F m -> In a dom -> m a <> None).
 Proof.
   unfold pred_domain.
   split.
+  - split; intros; repeat deex; eauto.
+    case_eq (m a); intros; eauto; firstorder.
   - split; intros.
     firstorder.
     intro.
     pose proof (H _ H0 a); firstorder.
     congruence.
-  - split; intros; repeat deex; eauto.
-    case_eq (m a); intros; eauto; firstorder.
 Qed.
+
+Hint Unfold pred_domain : pred.
+
+Ltac start := repeat autounfold with pred; intros; repeat deex; intuition;
+  repeat match goal with
+  | [ H: forall (_:mem), ?F _ -> _, H': ?F _ |- _ ] =>
+    learn that (H _ H')
+  end.
+
+Ltac dispatch := repeat split; intros;
+  repeat deex;
+  intuition eauto;
+  try congruence.
 
 Lemma exact_domain_oneside : forall F,
   (forall m1 m2, F m1 -> F m2 ->
     forall a, m1 a = None -> m2 a = None) ->
   exact_domain F.
 Proof.
-  unfold exact_domain.
-  split; intros; eauto.
+  start; dispatch.
 Qed.
 
 Remark pred_domain_exact_domain : forall F dom,
   pred_domain F dom -> exact_domain F.
 Proof.
-  intros; apply exact_domain_oneside; intros.
-  apply pred_domain_universal in H; destruct H.
+  start.
+  apply exact_domain_oneside; dispatch.
   destruct (in_dec AEQ a dom).
   firstorder.
   case_eq (m2 a); intros;
@@ -78,8 +91,8 @@ Lemma mem_union_some : forall m1 m2 a v,
   mem_union m1 m2 a = Some v ->
   m1 a = Some v \/ m2 a = Some v.
 Proof.
-  unfold mem_union; intros.
-  destruct (m1 a); eauto.
+  unfold mem_union; start.
+  destruct (m1 a); dispatch.
 Qed.
 
 Lemma mem_union_none : forall m1 m2 a,
@@ -87,7 +100,7 @@ Lemma mem_union_none : forall m1 m2 a,
   m1 a = None /\ m2 a = None.
 Proof.
   unfold mem_union; intros.
-  destruct (m1 a); eauto; congruence.
+  destruct (m1 a); dispatch.
 Qed.
 
 Theorem pred_domain_combine : forall F F' dom dom',
@@ -95,27 +108,86 @@ Theorem pred_domain_combine : forall F F' dom dom',
   pred_domain F' dom' ->
   pred_domain (F * F') (dom ++ dom').
 Proof.
-  unfold_sep_star.
-  intros.
-  rewrite pred_domain_universal in *; intuition; repeat deex.
+  unfold_sep_star; start; dispatch.
   eapply in_or_app.
-  destruct (mem_union_some _ _ H4); eauto.
+  destruct (mem_union_some _ _ H4); dispatch.
   eapply mem_union_none in H5; intuition.
-  eapply in_app_or in H4.
-  destruct H4; eauto.
+  destruct (in_app_or _ _ _ H4); dispatch.
 Qed.
 
 Theorem pred_domain_ptsto : forall a v,
   pred_domain (a |-> v) [a].
 Proof.
-  unfold ptsto; intros.
-  rewrite pred_domain_universal; intuition.
+  unfold ptsto; start.
   destruct (AEQ a a0); subst.
   constructor; auto.
-  specialize (H2 a0); intuition; congruence.
+  specialize (H1 a0); intuition; congruence.
 
-  inversion H0; subst; eauto.
-  specialize (H3 a0); intuition; congruence.
+  inversion H; subst; eauto.
+  specialize (H1 a0); dispatch.
+Qed.
+
+(* to learn something from pred_domain, need a memory to have
+F true, but F might be false in every memory *)
+Definition realizable F :=
+  exists m, F m.
+
+Lemma ptsto_single_mem : forall a v,
+  (a |-> v)%pred (@upd AT AEQ V empty_mem a v).
+Proof.
+  unfold ptsto, upd, empty_mem; start.
+  destruct (AEQ a a); dispatch.
+  unfold eq_rect_r.
+  rewrite <- Eqdep_dec.eq_rect_eq_dec; dispatch.
+
+  destruct (AEQ a' a); dispatch.
+Qed.
+
+Hint Unfold realizable : pred.
+
+Corollary realizable_ptsto : forall a v,
+  realizable (a |-> v).
+Proof.
+  unfold realizable; intros.
+  eauto using ptsto_single_mem.
+Qed.
+
+Theorem realizable_star_witness : forall F F' m,
+  (F * F')%pred m ->
+  realizable F.
+Proof.
+  unfold_sep_star; start; dispatch.
+Qed.
+
+Corollary realizable_star_witness' : forall F F' m,
+  (F * F')%pred m ->
+  realizable F'.
+Proof.
+  intros.
+  apply sep_star_comm in H.
+  eauto using realizable_star_witness.
+Qed.
+
+Theorem pred_domain_unique : forall F ls ls',
+  pred_domain F ls ->
+  pred_domain F ls' ->
+  (* must actually exist a mem in which F is true *)
+  realizable F ->
+  (forall a, In a ls -> In a ls').
+Proof.
+  start.
+
+  case_eq (m a); intros; dispatch.
+  firstorder.
+Qed.
+
+Theorem pred_domain_ptsto_in : forall F a v ls,
+  pred_domain (F * a |-> v) ls ->
+  realizable (F * a |-> v) ->
+  In a ls.
+Proof.
+  start; dispatch.
+  eauto using ptsto_valid'.
 Qed.
 
 (* at least the locks in dom are held *)
@@ -134,6 +206,30 @@ Definition split_frames tid F LF (ls: list AT) : S -> Prop :=
     (F * LF)%pred (proj s) /\
     pred_domain LF ls /\
     locked tid ls s.
+
+Hint Unfold split_frames locked : pred.
+
+Theorem split_frame_ptsto_locked : forall tid F LF a v ls s,
+  split_frames tid F (LF * a |-> v) ls s ->
+  lock s a = Owned tid.
+Proof.
+  start; dispatch.
+  unfold sep_star in H0 at 1.
+  rewrite sep_star_is in H0.
+  unfold sep_star_impl in H0.
+  repeat deex.
+
+  eauto using ptsto_valid'.
+Qed.
+
+Theorem split_frame_indifferent : forall tid F LF ls s s',
+  split_frames tid F LF ls s ->
+  (forall a, lock s a = Owned tid -> lock s' a = Owned tid) ->
+  proj s' = proj s ->
+  split_frames tid F LF ls s'.
+Proof.
+  start; dispatch.
+Qed.
 
 End State.
 
